Use new libraries on all files. Perform some renaming...

sha3/proof/old/IndifPadding.ec
@@ -4,8 +4,7 @@ require (*..*) Indifferentiability LazyRO.
 clone import Indifferentiability as Ind1.
 
 clone import Indifferentiability as Ind2
-  with type p_in  <- Ind1.p_in,
-       type p_out <- Ind1.p_out,
+  with type p  <- Ind1.p,
        type f_out <- Ind1.f_out.
 
 op pad : Ind2.f_in -> Ind1.f_in.
@@ -22,25 +21,25 @@ clone import LazyRO as RO2
        type to   <- Ind1.f_out,
        op d      <- RO1.d.
 
-module ConstrPad (FC:Ind1.Construction, P:Ind1.Primitive) = {
+module ConstrPad (FC:Ind1.CONSTRUCTION, P:Ind1.PRIMITIVE) = {
   module C = FC(P)
 
   proc init = C.init
 
-  proc oracle (x:Ind2.f_in) : f_out = {
+  proc f (x:Ind2.f_in) : f_out = {
     var r;
-    r = C.oracle(pad x);
+    r = C.f(pad x);
     return r;
   }
 }.
 
-module DistPad(FD: Ind2.Distinguisher, F:Ind1.Functionality, P:Ind1.Primitive) = {
+module DistPad(FD: Ind2.DISTINGUISHER, F:Ind1.FUNCTIONALITY, P:Ind1.PRIMITIVE) = {
   module Fpad = {
     proc init = F.init
 
-    proc oracle(x:Ind2.f_in) : f_out = {
+    proc f(x:Ind2.f_in) : f_out = {
       var r;
-      r = F.oracle(pad x);
+      r = F.f(pad x);
       return r;
     }
   }
@@ -48,12 +47,12 @@ module DistPad(FD: Ind2.Distinguisher, F:Ind1.Functionality, P:Ind1.Primitive) =
   proc distinguish = FD(Fpad,P).distinguish
 }.
 
-module SimPadinv(S:Ind1.Simulator, F2:Ind2.Functionality) = {
+module SimPadinv(S:Ind1.SIMULATOR, F2:Ind2.FUNCTIONALITY) = {
   module F1 = {
     proc init = F2.init
-    proc oracle(x:Ind1.f_in):Ind1.f_out = {
+    proc f(x:Ind1.f_in):Ind1.f_out = {
       var r;
-      r = F2.oracle(padinv x);
+      r = F2.f(padinv x);
       return r;
     }
   }
@@ -62,30 +61,31 @@ module SimPadinv(S:Ind1.Simulator, F2:Ind2.Functionality) = {
 
   proc init = S2.init
 
-  proc oracle = S2.oracle
+  proc f = S2.f
+  proc fi = S2.fi
 }.
 
 section Reduction.
-  declare module P  : Ind1.Primitive. (* It is compatible with Ind2.Primitive *)  
-  declare module C  : Ind1.Construction {P}.
-  declare module S  : Ind1.Simulator{ RO1.H, RO2.H}.
+  declare module P  : Ind1.PRIMITIVE. (* It is compatible with Ind2.Primitive *)  
+  declare module C  : Ind1.CONSTRUCTION {P}.
+  declare module S  : Ind1.SIMULATOR{ RO1.H, RO2.H}.
 
-  declare module D' : Ind2.Distinguisher{P,C, RO1.H, RO2.H, S}.
+  declare module D' : Ind2.DISTINGUISHER{P,C, RO1.H, RO2.H, S}.
 
   local equiv ConstrDistPad: 
-      Ind2.Real(P, ConstrPad(C), D').main ~ 
-      Ind1.Real(P, C, DistPad(D')).main : ={glob P, glob C, glob D'} ==> 
+      Ind2.GReal(ConstrPad(C), P, D').main ~ 
+      Ind1.GReal(C, P, DistPad(D')).main : ={glob P, glob C, glob D'} ==> 
                                               ={glob P, glob C, glob D', res}.
   proof. by sim. qed.
 
   local lemma PrConstrDistPad &m: 
-      Pr[ Ind2.Real(P,ConstrPad(C), D').main() @ &m : res] =
-      Pr[ Ind1.Real(P,C,DistPad(D')).main() @ &m : res].
+      Pr[ Ind2.GReal(ConstrPad(C), P, D').main() @ &m : res] =
+      Pr[ Ind1.GReal(C, P, DistPad(D')).main() @ &m : res].
   proof. by byequiv ConstrDistPad. qed.
 
   local equiv DistH2H1:
-      Ind2.Ideal(RO2.H, SimPadinv(S), D').main ~
-      Ind1.Ideal(RO1.H, S, DistPad(D')).main :
+      Ind2.GIdeal(RO2.H, SimPadinv(S), D').main ~
+      Ind1.GIdeal(RO1.H, S, DistPad(D')).main :
         ={glob D', glob S} ==>
         ={glob D',glob S, res} /\ forall x, RO2.H.m{1}.[padinv x] = RO1.H.m{2}.[x].
   proof.
@@ -96,25 +96,31 @@ section Reduction.
       proc;inline *;wp;sp;if;first by progress [-split];rewrite !in_dom H.
       + auto;progress;first by rewrite !getP_eq.
         by rewrite !getP (can_eq _ _ cancel_padinv) H.
+      by auto;progress;rewrite H. 
+    + proc *;inline *.
+      call (_: forall x, RO2.H.m{1}.[padinv x] = RO1.H.m{2}.[x]);auto.
+      proc;inline *;wp;sp;if;first by progress [-split];rewrite !in_dom H.
+      + auto;progress;first by rewrite !getP_eq.
+        by rewrite !getP (can_eq _ _ cancel_padinv) H.
       by auto;progress;rewrite H.      
     + proc;inline *;wp;sp;if;first by progress[-split];rewrite -{1}(cancel_pad x{2}) !in_dom H.
       + auto;progress;first by rewrite !getP_eq.  
         by rewrite !getP (eq_sym x1) (can2_eq _ _ cancel_pad cancel_padinv) (eq_sym x{2}) H.
       by auto;progress;rewrite -H cancel_pad.
-    inline *;wp. call (_: ={glob D'});first by sim.
+    inline *;wp. call (_: ={glob D'}). 
     auto;progress;by rewrite !map0P.
   qed.
 
   local lemma PrDistH2H1 &m:  
-      Pr[Ind2.Ideal(RO2.H,SimPadinv(S),D').main() @ &m : res] =
-      Pr[Ind1.Ideal(RO1.H,S, DistPad(D')).main() @ &m : res].
+      Pr[Ind2.GIdeal(RO2.H,SimPadinv(S),D').main() @ &m : res] =
+      Pr[Ind1.GIdeal(RO1.H,S, DistPad(D')).main() @ &m : res].
   proof. by byequiv DistH2H1. qed.
 
   lemma Conclusion &m:
-      `| Pr[Ind2.Real (P  , ConstrPad(C), D').main() @ &m : res] -
-         Pr[Ind2.Ideal(RO2.H, SimPadinv(S), D').main() @ &m : res] | =
-      `| Pr[Ind1.Real(P   , C, DistPad(D')).main() @ &m : res] - 
-         Pr[Ind1.Ideal(RO1.H, S, DistPad(D')).main() @ &m : res] |.
+      `| Pr[Ind2.GReal (ConstrPad(C), P           , D'         ).main() @ &m : res] -
+         Pr[Ind2.GIdeal(RO2.H       , SimPadinv(S), D'         ).main() @ &m : res] | =
+      `| Pr[Ind1.GReal (C           , P           , DistPad(D')).main() @ &m : res] - 
+         Pr[Ind1.GIdeal(RO1.H       , S           , DistPad(D')).main() @ &m : res] |.
   proof. by rewrite (PrConstrDistPad &m) (PrDistH2H1 &m). qed.
 
 end section Reduction.
